PSLCore/Try_Hard.thy
@@ -1,29 +1,27 @@
-theory Try_Hard
+theory Try_Hard 
 imports Isar_Interface
 begin
 
-strategy TryHard = 
-  Ors [Thens [Auto, IsSolved],
-       Thens [Induct, Auto, IsSolved],
+strategy TryHard =
+  Ors [
+       Thens [Auto, IsSolved],
+       Thens [IntroClasses, Auto, IsSolved],
+       Thens [Transfer, Auto, IsSolved],
+       Thens [Normalization, IsSolved],
+       Thens [Hammer, IsSolved],
        Thens [Dynamic (Induct), Auto, IsSolved],
-       Thens [Repeat (Ors [Fastforce,
-                           Hammer,
-                           Thens [Clarsimp, Hammer]]),
+       Thens [Dynamic (Cases), Auto, IsSolved],
+       Thens [Dynamic (Auto), IsSolved],
+       Thens [Dynamic (Coinduction), Auto, IsSolved],
+       Thens [Repeat (Ors [Fastforce, Hammer]), IsSolved],
+       Thens [Dynamic (Cases), Repeat (Ors [Fastforce, Hammer]), IsSolved],
+       Thens [IntroClasses,
+              Repeat (Ors [Fastforce, Thens [Transfer, Fastforce], Hammer]),
               IsSolved],
-       Thens [Case, Auto, IsSolved],
-       Thens [Dynamic ( Simp ), IsSolved],
-       Thens [Case,
-              Repeat (Ors [Hammer,
-                           Fastforce,
-                           Thens [Clarsimp, Hammer]]),
-              IsSolved],
-       Thens [Dynamic (Induct),
-              Repeat (Ors [Fastforce,
-                           Hammer,
-                           Thens [Clarsimp, Hammer]]),
-              IsSolved]
+       Thens [Transfer, Repeat (Ors [Fastforce, Hammer]), IsSolved],
+       Thens [Dynamic (Induct), Repeat (Ors [Fastforce, Hammer]), IsSolved]
        ]
-  
+
 lemma "True" and "True"
 try_hard
 oops
