Runtime/Dynamic_Cases.thy
@@ -1,0 +1,62 @@
+(* This file provides a mechanism to generate cases tactics dynamically, utilising run-time
+ * information.*)
+theory Dynamic_Cases
+imports
+  Dynamic_Tactic_Generation
+  "../Utils/More_Find_Theorems"
+begin
+
+ML{* structure Cases_Seed : DYNAMIC_TACTIC_GENERATOR_SEED =
+struct
+
+datatype modifier = On of string;
+
+type modifiers = modifier list;
+
+fun get_ons   (fvars:string list) = map On fvars;
+
+fun order (mods:modifiers) = mods;
+
+fun get_name (On name) = name;
+
+val get_names = map get_name;
+
+fun mods_to_string (mods:modifiers) =
+    mods |> order |> (fn ons => get_names ons |> Dynamic_Utils.get_meth_nm "");
+
+fun get_all_modifiers (state:Proof.state) =
+  let
+    val {goal: thm,...} = Proof.goal state;
+    val free_var_names   = Isabelle_Utils.get_free_var_names_in_thm goal;
+    val all_cases_mods  = get_ons free_var_names;
+  in
+    all_cases_mods : modifiers
+  end;
+
+end;
+*}
+
+ML{* structure Cases_Tactic_Generator : DYNAMIC_TACTIC_GENERATOR = 
+  mk_Dynamic_Tactic_Generator (Cases_Seed);
+*}
+
+ML{* structure Dynamic_Cases : DYNAMIC_TACTIC =
+struct
+
+structure CTG = Cases_Tactic_Generator;
+
+fun get_state_stttacs (state:Proof.state) =
+  let
+    val induct         = "cases";
+    val all_modifiers  = CTG.get_all_modifiers state : CTG.modifiers;
+    val all_modifierss   = map single all_modifiers |> Seq.of_list : CTG.modifiers Seq.seq;
+    val stttacs        = Seq.map (CTG.meth_name_n_modifiers_to_stttac_on_state induct) all_modifierss;
+    type 'a stttac = 'a Dynamic_Utils.stttac;
+  in 
+    stttacs : Proof.state stttac Seq.seq
+  end;
+
+end;
+*}
+
+end
