ROOT
@@ -2,7 +2,7 @@ session "PSL" = "HOL" +
   options [document = pdf, document_output = "output", timeout = 600]
   theories [document = false]
   theories
-    "Example"
+    "PSL"
   document_files
     "root.tex"
     "root.bib"
